extraction/Extract.v
@@ -1,5 +1,5 @@
 From PackageCalculus Require Import Prelude Core Versions Conflict Visibility
-  Smoke.
+  Debian Smoke.
 From Stdlib Require Import Extraction ExtrOcamlBasic.
 
 Extraction Language OCaml.
@@ -16,4 +16,5 @@ Set Warnings "-extraction-opaque-accessed".
 
 Extraction "pac_extraction.ml"
   Smoke.C Smoke.Ver Smoke.Cfl Smoke.Conc Smoke.Peer Smoke.Vis
-  Smoke.Feat Smoke.Virt Smoke.PkgF Smoke.VarF Smoke.FC.
+  Smoke.Feat Smoke.Virt Smoke.PkgF Smoke.VarF Smoke.FC
+  Debian.
